Start fixing `sync` proofs

trusted/sync.v
@@ -4,12 +4,25 @@ Section code.
 Context `{ext_ty: ext_types}.
 Local Coercion Var' s: expr := Var s.
 
+(* FIXME: make everything in here opaque. *)
+
 (* FIXME: want to expose a type, not descriptor *)
-Axiom Mutex : descriptor.
+Definition Mutex : descriptor :=
+  ["state" :: boolT]
+.
 Axiom WaitGroup: descriptor.
 
-Axiom Mutex__Lock : val.
-Axiom Mutex__Unlock : val.
+Definition Mutex__Lock : val :=
+  rec: "f" "m" :=
+    if: CmpXchg (struct.fieldRef Mutex "state" "m") #false #true then
+      #()
+    else
+      "f" #()
+.
+Definition Mutex__Unlock : val :=
+  λ: "f" "m", CmpXchg (struct.fieldRef Mutex "state" "m") #true #false
+.
+
 Axiom NewCond: val.
 Axiom Cond__Wait: val.
 Axiom Cond__Broadcast: val.
