src/program_proof/sync.v
@@ -1,0 +1,263 @@
+From stdpp Require Import namespaces.
+From iris.proofmode Require Import tactics.
+From iris.algebra Require Import excl.
+From Perennial.base_logic.lib Require Import invariants.
+From Perennial.program_logic Require Import weakestpre.
+
+From Perennial.goose_lang Require Import lang typing.
+From Perennial.goose_lang Require Import proofmode notation.
+From Perennial.goose_lang Require Import persistent_readonly.
+From Perennial.goose_lang.lib Require Import typed_mem.
+From Goose Require Export sync.
+From Perennial.program_proof Require Import grove_prelude.
+Set Default Proof Using "Type".
+
+Section goose_lang.
+Context `{ffi_sem: ffi_semantics}.
+Context `{!ffi_interp ffi}.
+Context {ext_tys: ext_types ext}.
+
+Local Coercion Var' (s:string): expr := Var s.
+
+Section proof.
+  Context `{!heapGS Σ} (N : namespace).
+
+  (** This means [m] is a valid mutex with invariant R. *)
+  Definition is_Mutex (m: loc) (R : iProp Σ) : iProp Σ :=
+    inv N (
+          ∃ b : bool, m ↦[Mutex :: "state"]{1/4} #b ∗
+                   if b then True else m ↦[Mutex :: "state"]{3/4} #b ∗ R
+          ).
+
+  (** This resource denotes ownership of the lock (i.e. the lock is currently
+      held). *)
+  Definition own_Mutex (m: loc) : iProp Σ := m ↦[Mutex :: "state"]{3/4} #true.
+
+  Lemma own_Mutex_exclusive (m : loc) : own_Mutex m -∗ own_Mutex m -∗ False.
+  Proof.
+    iIntros "H1 H2".
+    iCombine "H1 H2" as "H".
+    (* FIXME: need
+    iDestruct (struct_field_pointsto_frac_valid with "H") as %Hval. *)
+    admit.
+  Admitted.
+
+  Global Instance is_Mutex_ne m : NonExpansive (is_Mutex m).
+  Proof. solve_proper. Qed.
+
+  (** The main proofs. *)
+  Global Instance is_Mutex_persistent m R : Persistent (is_Mutex m R).
+  Proof. apply _. Qed.
+  Global Instance locked_timeless m : Timeless (own_Mutex m).
+  Proof. apply _. Qed.
+
+  (** Denotes ownership of a mutex for which the lock invariant is not yet
+      decided *)
+  Definition own_uninit_Mutex (m: loc): iProp Σ := m ↦[Mutex :: "state"] #false.
+
+  Theorem init_Mutex_inv R E m : own_uninit_Mutex m -∗ ▷ R ={E}=∗ is_Mutex m R.
+  Proof.
+    iIntros "Hl HR".
+    iMod (inv_alloc N _ (_) with "[Hl HR]") as "#?".
+    2:{ by iFrame "#". }
+    { iIntros "!>". iExists false. iFrame.
+      rewrite /own_uninit_Mutex.
+      iEval (rewrite -Qp.quarter_three_quarter) in "Hl".
+      iDestruct "Hl" as "[Hl1 Hl2]".
+      iFrame.
+    }
+  Qed.
+
+  (* FIXME: lemma for (zero_val Mutex) *)
+  (*
+  Lemma wp_new_free_lock E:
+    {{{ True }}} lock.new #() @ E {{{ m, RET #lk; own_uninit_Mutex m }}}.
+  Proof.
+    iIntros (Φ) "_ HΦ".
+    wp_call.
+    wp_apply wp_alloc_untyped; auto.
+  Qed. *)
+
+  (*
+  Lemma newlock_spec E (R : iProp Σ):
+    {{{ ▷ R }}} lock.new #() @ E {{{ (lk:loc), RET #lk; own_lock #lk R }}}.
+  Proof.
+    iIntros (Φ) "HR HΦ". rewrite -wp_fupd /lock.new /=.
+    wp_lam. wp_apply wp_alloc_untyped; first by auto.
+    iIntros (l) "Hl".
+    iMod (alloc_lock with "[$] HR") as "Hlock".
+    iModIntro.
+    iApply "HΦ". iFrame.
+  Qed. *)
+
+  Lemma wp_Mutex__Lock m R :
+    {{{ is_Mutex m R }}}
+      Mutex__Lock #m
+    {{{ RET #(); own_Mutex m ∗ R }}}.
+  Proof.
+    iIntros (Φ) "#Hinv HΦ".
+    wp_rec.
+    wp_apply wp_struct_fieldRef; first done.
+    wp_bind (CmpXchg _ _ _).
+    wp_pures.
+    iInv N as ([]) "[Hl HR]".
+    -
+      (* FIXME: struct fieldRef_f should match up with struct field points-tos. *)
+      wp_cmpxchg_fail. iModIntro. iSplitL "Hl"; first (iNext; iExists true; eauto).
+      wp_pures. iApply ("HΦ" $! false). done.
+    - iDestruct "HR" as "[Hl2 HR]".
+      iCombine "Hl Hl2" as "Hl".
+      rewrite Qp.quarter_three_quarter.
+      wp_cmpxchg_suc.
+      iModIntro.
+      iEval (rewrite -Qp.quarter_three_quarter) in "Hl".
+      iDestruct "Hl" as "[Hl1 Hl2]".
+      iSplitL "Hl1"; first (iNext; iExists true; eauto).
+      rewrite /locked. wp_pures.
+      iApply "HΦ".
+      eauto with iFrame.
+  Qed.
+
+  Lemma acquire_spec' stk E lk R :
+    ↑N ⊆ E →
+    {{{ is_lock lk R }}} lock.acquire lk @ stk; E {{{ RET #(); locked lk ∗ R }}}.
+  Proof.
+    iIntros (? Φ) "#Hl HΦ". iLöb as "IH". wp_rec.
+    wp_apply (try_acquire_spec with "Hl"); auto. iIntros ([]).
+    - iIntros "[Hlked HR]". wp_if. iApply "HΦ"; by iFrame.
+    - iIntros "_". wp_if. iApply ("IH" with "[HΦ]"). auto.
+  Qed.
+
+  Lemma acquire_spec lk R :
+    {{{ is_lock lk R }}} lock.acquire lk {{{ RET #(); locked lk ∗ R }}}.
+  Proof. eapply acquire_spec'; auto. Qed.
+
+  Lemma release_spec' stk E lk R :
+    ↑N ⊆ E →
+    {{{ is_lock lk R ∗ locked lk ∗ ▷ R }}} lock.release lk @ stk; E {{{ RET #(); True }}}.
+  Proof.
+    iIntros (? Φ) "(Hlock & Hlocked & HR) HΦ".
+    iDestruct "Hlock" as (l ->) "#Hinv".
+    rewrite /lock.release /=. wp_lam.
+    wp_bind (CmpXchg _ _ _).
+    iInv N as (b) "[>Hl _]".
+
+    iDestruct (locked_loc with "Hlocked") as "Hl2".
+    iDestruct (heap_pointsto_agree with "[$Hl $Hl2]") as %->.
+    iCombine "Hl Hl2" as "Hl".
+    rewrite Qp.quarter_three_quarter.
+    wp_cmpxchg_suc.
+    iModIntro.
+    iSplitR "HΦ"; last by wp_seq; iApply "HΦ".
+    iEval (rewrite -Qp.quarter_three_quarter) in "Hl".
+    iDestruct "Hl" as "[Hl1 Hl2]".
+    iNext. iExists false. iFrame.
+  Qed.
+
+  Lemma release_spec lk R :
+    {{{ is_lock lk R ∗ locked lk ∗ ▷ R }}} lock.release lk {{{ RET #(); True }}}.
+  Proof. eapply release_spec'; auto. Qed.
+
+  Lemma release_spec'' lk R :
+    is_lock lk R -∗ {{{ locked lk ∗ ▷ R }}} lock.release lk {{{ RET #(); True }}}.
+  Proof.
+    iIntros "#Hlock !# %Φ [??] HΦ". iApply (release_spec with "[-HΦ]"); by iFrame.
+  Qed.
+
+  (** cond var proofs *)
+
+  Definition is_cond (c: loc) (lk : val) : iProp Σ :=
+    readonly (c ↦ lk).
+
+  Global Instance is_cond_persistent c lk :
+    Persistent (is_cond c lk) := _.
+
+  Theorem wp_newCond' lk :
+    {{{ is_free_lock lk }}}
+      lock.newCond #lk
+    {{{ (c: loc), RET #c; is_free_lock lk ∗ is_cond c #lk }}}.
+  Proof.
+    rewrite /is_cond.
+    iIntros (Φ) "Hl HΦ".
+    wp_call.
+    wp_apply wp_alloc_untyped; [ auto | ].
+    iIntros (c) "Hc".
+    (* FIXME: need a let binding in the implementation to do an iMod after the
+    Alloc (so the goal needs to still be a WP) *)
+    iMod (readonly_alloc_1 with "Hc") as "Hcond".
+    wp_pures.
+    iApply "HΦ". by iFrame.
+  Qed.
+
+  Theorem wp_newCond lk R :
+    {{{ is_lock lk R }}}
+      lock.newCond lk
+    {{{ (c: loc), RET #c; is_cond c lk }}}.
+  Proof.
+    rewrite /is_cond.
+    iIntros (Φ) "Hl HΦ".
+    wp_call.
+    iDestruct (is_lock_flat with "Hl") as %[l ->].
+    wp_apply wp_alloc_untyped; [ auto | ].
+    iIntros (c) "Hc".
+    (* FIXME: need a let binding in the implementation to do an iMod after the
+    Alloc (so the goal needs to still be a WP) *)
+    iMod (readonly_alloc_1 with "Hc") as "Hcond".
+    wp_pures.
+    by iApply "HΦ".
+  Qed.
+
+  Theorem wp_condSignal c lk :
+    {{{ is_cond c lk }}}
+      lock.condSignal #c
+    {{{ RET #(); True }}}.
+  Proof.
+    iIntros (Φ) "Hc HΦ".
+    wp_call.
+    iApply ("HΦ" with "[//]").
+  Qed.
+
+  Theorem wp_condBroadcast c lk :
+    {{{ is_cond c lk }}}
+      lock.condBroadcast #c
+    {{{ RET #(); True }}}.
+  Proof.
+    iIntros (Φ) "Hc HΦ".
+    wp_call.
+    iApply ("HΦ" with "[//]").
+  Qed.
+
+  Theorem wp_condWait c lk R :
+    {{{ is_cond c lk ∗ is_lock lk R ∗ locked lk ∗ R }}}
+      lock.condWait #c
+    {{{ RET #(); locked lk ∗ R }}}.
+  Proof.
+    iIntros (Φ) "(#Hcond&#Hlock&Hlocked&HR) HΦ".
+    wp_call.
+    rewrite /is_cond.
+    iMod (readonly_load with "Hcond") as (q) "Hc".
+    wp_untyped_load.
+    wp_apply (release_spec with "[$Hlock $Hlocked $HR]").
+    wp_pures.
+    wp_untyped_load.
+    wp_apply (acquire_spec with "[$Hlock]").
+    iIntros "(Hlocked&HR)".
+    iApply "HΦ".
+    iFrame.
+  Qed.
+
+  Theorem wp_condWaitTimeout c (t : u64) lk R :
+    {{{ is_cond c lk ∗ is_lock lk R ∗ locked lk ∗ R }}}
+      lock.condWaitTimeout #c #t
+    {{{ RET #(); locked lk ∗ R }}}.
+  Proof.
+    iIntros (Φ) "Hpre HΦ".
+    wp_lam. wp_pures.
+    wp_apply (wp_condWait with "Hpre").
+    done.
+  Qed.
+
+End proof.
+End goose_lang.
+
+(* Typeclasses Opaque is_lock is_cond locked. *)
